\documentclass{article}
\usepackage[utf8]{inputenc}
\usepackage{amsmath}
\title{fjiowaefjio}
\author{1983nianxiaoxiang}
\date{October 2019}


\begin{document}\large
Assume the load factor is $ \alpha = \frac{m}{n} $, the random variable $X$ denotes the number of slots hit until an empty slot.
Assume $n >= m+3$

$$P(X = k) = \frac{\binom{n-k}{m-k+1}}{\binom{n}{m}}\\ $$

$$E(X) = \Sigma_{k = 1}^{m + 1} kP(X = k)\\$$
$$= \frac{\Sigma_{k = 1}^{m+1}k\binom{n-k}{m-k+1}}{\binom{n}{m}}\\$$
$$= \frac{\Sigma_{l = 1}^{m+1}\Sigma_{k = l}^{m+1}\binom{n-k}{m-k+1}}{\binom{n}{m}}$$
$$= \frac{\Sigma_{l = 1}^{m+1}\Sigma_{k = l}^{m+1}\binom{n-k}{m-k+1}}{\binom{n}{m}}$$
$$= \frac{\Sigma_{l = 1}^{m+1}\Sigma_{t = 0}^{m+1-l}\binom{n-m-1+t}{t}}{\binom{n}{m}}$$   

As we have $$\binom{n-1}{k-1} + \binom{n-1}{k} = \binom{n}{k}$$,
$$\Sigma_{t = 0}^{m+1-l}\binom{n-m-1+t}{t}$$
$$= \binom{n-m-1}{0} + \binom{n-m}{1} + ... + \binom{n-l}{m-1+l}$$
$$= \binom{n-m-1}{0} - \binom{n-m-1}{1} + \binom{n-m-1}{1} + \binom{n-m}{1} + ... + \binom{n-l}{m-1+l}$$
$$= \binom{n-m-1}{0} - \binom{n-m-1}{1} + \binom{n-l}{m+2-l}$$
$$= m+2-n + \binom{n-l}{m+2-l}$$
Again, we use the same trick, and we get
$$\Sigma_{l = 1}^{m+1}\Sigma_{t = 0}^{m+1-l}\binom{n-m-1+t}{t}$$  
$$ = n(m+2-n)+1-\frac{(n-m-1)(n-m)}{2}+\binom{n-1}{m+2}$$
$$ E(X) = O(\frac{\binom{n-1}{m+2}}{\binom{n}{m}})$$
$$=O(\frac{\frac{(n-1)!}{(m+2)!(n-m-3)!}}{\frac{n!}{(n-m)!m!}})$$
$$=O(\frac{(1-\alpha)n((1-\alpha)n-1)((1-\alpha)n-2)}{n(\alpha n+1)(\alpha n+2)})$$
$$=O(\frac{(1-\alpha)^{2}n}{\alpha^{2} n}) = O(1)$$















\end{document}


